modified:   coq/cpdt/chapt2.v

coq/cpdt/chapt2.v
@@ -1,99 +1,130 @@
-Set Implicit Arguments.
+Require Import Coq.Lists.List.
 
-Require Import List.
-Require Import Bool.
-Require Import Arith.
-
-
-Inductive binop : Set := Plus | Times.
+Inductive binop : Set := 
+| Plus  : binop
+| Times : binop
+.
 
 Inductive exp : Set :=
-    | Const : nat -> exp
-    | Binop : binop -> exp -> exp -> exp
-    .
-
+| Const : nat -> exp
+| Binop : binop -> exp-> exp -> exp
+.
 
 Definition binopDenote (b:binop) : nat -> nat -> nat :=
+    match b with 
+    | Plus  => plus
+    | Times => mult
+    end.
+
+(* type inference at play *) 
+Definition binopDenote' := fun b => 
     match b with
-        | Plus  => plus
-        | Times => mult
+    | Plus  => plus
+    | Times => mult
     end.
 
 Fixpoint expDenote (e:exp) : nat :=
     match e with
-        | Const n       => n
-        | Binop b e1 e2 => binopDenote b (expDenote e1) (expDenote e2)
+    | Const n       => n
+    | Binop b e1 e2 => binopDenote b (expDenote e1) (expDenote e2)
     end.
 
+(*
 Compute expDenote (Const 42).
 Compute expDenote (Binop Plus (Const 2) (Const 3)).
 Compute expDenote (Binop Times (Binop Plus (Const 2) (Const 3)) (Const 7)).
+*)
 
+Lemma expDenote_test1 : expDenote (Const 42) = 42.
+Proof. reflexivity. Qed.
+
+Lemma expDenote_test2 : expDenote (Binop Plus (Const 2) (Const 3)) = 5.
+Proof. reflexivity. Qed.
+
+Lemma expDenote_test3 : expDenote (Binop Times (Binop Plus (Const 2) (Const 3)) (Const 7)) = 35.
+Proof. reflexivity. Qed.
 
 Inductive instr : Set :=
-    | iConst : nat -> instr
-    | iBinop : binop -> instr    
-    .
+| iConst : nat   -> instr
+| iBinop : binop -> instr
+.
 
-Definition prog  := list instr.
-Definition stack := list nat.
+Definition prog  : Set := list instr.
+Definition stack : Set := list nat.
 
-Definition instrDenote (i:instr)(s:stack) : option stack :=
+Definition instrDenote (i:instr) (s:stack) : option stack :=
     match i with
-        | iConst n  => Some (n::s)
-        | iBinop b  => 
-            match s with
-                | arg1 :: arg2 :: s' => Some (binopDenote b arg1 arg2 :: s') 
-                | _                  => None
-            end
-    end.
-             
-Fixpoint progDenote (p:prog)(s:stack) : option stack :=
-    match p with
-        | nil   => Some s
-        | i::p' => 
-            match instrDenote i s with
-                | None    => None
-                | Some s' => progDenote p' s'
-            end
+    | iConst n  => Some (n :: s)
+    | iBinop b  => 
+        match s with
+        | x1 :: x2 :: s'    => Some ((binopDenote b) x1 x2 :: s')
+        | _                 => None
+        end
     end.
 
+Fixpoint progDenote (p:prog) (s:stack) : option stack :=
+    match p with
+    | nil       => Some s
+    | i :: q    => 
+        match instrDenote i s with
+        | None      => None
+        | Some s'   => progDenote q s'
+        end
+    end.
 
 Fixpoint compile (e:exp) : prog :=
     match e with
-        | Const n       => iConst n :: nil
-        | Binop b e1 e2 => compile e2 ++ compile e1 ++ iBinop b :: nil
+    | Const n       => iConst n :: nil
+    | Binop b e1 e2 => compile e2 ++ compile e1 ++ iBinop b :: nil
     end.
 
-Compute compile (Const 42).
-Compute compile (Binop Plus (Const 2) (Const 3)).
-Compute compile (Binop Times (Binop Plus (Const 2) (Const 3)) (Const 7)).
 
-Compute progDenote (compile (Const 42)) nil.
-Compute progDenote (compile (Binop Plus (Const 2) (Const 3))) nil.
-Compute progDenote (
-    compile (Binop Times (Binop Plus (Const 2) (Const 3)) (Const 7))) nil.
+Lemma compile_test1 : compile (Const 42) = iConst 42 :: nil.
+Proof. reflexivity. Qed.
+
+Lemma compile_test2 : compile (Binop Plus (Const 2) (Const 3)) 
+    = iConst 3 :: iConst 2 :: iBinop Plus :: nil
+    .
+Proof. reflexivity. Qed.
+
+Lemma compile_test3 : compile (Binop Times (Binop Plus (Const 2) (Const 3)) (Const 7)) 
+    = iConst 7 :: iConst 3 :: iConst 2 :: iBinop Plus :: iBinop Times :: nil
+    .
+Proof. reflexivity. Qed.
+
+Definition eval (e:exp) : option nat :=
+    match progDenote (compile e) nil with
+    | Some (n::nil) => Some n
+    | _             => None
+    end.
+
+Lemma eval_test1 : eval (Const 42) = Some 42.
+Proof. reflexivity. Qed.
+
+Lemma eval_test2 : eval (Binop Plus (Const 2) (Const 3)) = Some 5.
+Proof. reflexivity. Qed.
+    
+Lemma eval_test3 : eval (Binop Times (Binop Plus (Const 2) (Const 3)) (Const 7)) = Some 35.
+Proof. reflexivity. Qed.
 
 
-Lemma correctness' : forall e p s,
+Lemma compile_correct' : forall (e:exp) (p:prog) (s:stack),
     progDenote (compile e ++ p) s = progDenote p (expDenote e :: s).
 Proof.
-    intros e. elim e.
-    clear e. intros n p s. simpl. reflexivity.
-    clear e. intros b. intros e1 H1 e2 H2 p s. simpl.
-    rewrite app_assoc_reverse. rewrite H2.
-    rewrite app_assoc_reverse. rewrite H1.
-    simpl. reflexivity.
+    intros e. induction e as [n|b e1 H1 e2 H2]; intros p s; simpl.
+    - reflexivity.
+    - rewrite app_assoc_reverse. rewrite H2. 
+      rewrite app_assoc_reverse. rewrite H1.
+      reflexivity.
 Qed.
 
-
-Theorem correctness : forall e, 
-    progDenote (compile e) nil = Some (expDenote e ::nil).
+Theorem compile_correct : forall (e:exp), eval e = Some (expDenote e).
 Proof.
-    intros e. rewrite app_nil_end with (l:=compile e). apply correctness'.
+    intros e. unfold eval. rewrite <- (app_nil_r (compile e)).
+    rewrite compile_correct'. reflexivity.
 Qed.
 
-
+(*
 
 Inductive type : Set := Nat | Bool.
 
@@ -152,7 +183,7 @@ Compute texpDenote (TBinop TLt
     (TBinop TPlus (TNConst 2) (TNConst 2))
     (TNConst 4)).
 
-
+*)
 
 
 
